UntypedComp: prove compilation commutes with subst

src/UntypedComp.v
@@ -1,5 +1,7 @@
-Require Import List.
+Require Import List Arith Omega.
 Import ListNotations.
+
+Require Import StructTact.StructTactics.
 
 Require SourceLang.
 Require Untyped.
@@ -37,7 +39,7 @@ Definition elim_to_type_name {l cases target} (e : S.elim l cases target) : U.ty
   | S.EListNat _ => U.Tlist_nat
   end.
 
-Definition expr {l ty} (e : S.expr l ty) : U.expr :=
+Definition compile {l ty} (e : S.expr l ty) : U.expr :=
   let fix go {l ty} (e : S.expr l ty) : U.expr :=
       let fix go_hlist {l tys} (h : S.hlist (S.expr l) tys) : list U.expr :=
           match h with
@@ -53,3 +55,92 @@ Definition expr {l ty} (e : S.expr l ty) : U.expr :=
       | S.Elim e cases target => U.Elim (elim_to_type_name e) (go_hlist cases) (go target)
       end
   in go e.
+
+Fixpoint hmap_simple {A} {B : A -> Type} {C l} (f : forall a, B a -> C) (h : S.hlist B l) : list C :=
+  match h with
+  | S.hnil => []
+  | S.hcons x h' => cons (f _ x) (hmap_simple f h')
+  end.
+
+Require Import Program.
+
+Lemma nth_member_hget :
+  forall A (B : A -> Type) C (f : forall a, B a -> C) c l (h : S.hlist B l) t (m : S.member t l),
+    nth (member m) (hmap_simple f h) c = f _ (S.hget h m).
+Proof.
+  induction h; intros; dependent destruction m; simpl; auto.
+Qed.
+
+
+Lemma member_insert_member :
+  forall A (a1 a2 : A) l (m : S.member a1 l) n,
+    member (S.insert_member(ty' := a2) m n) =
+    if Compare_dec.lt_dec (member m) n then member m else S (member m).
+Proof.
+  induction m; simpl; intros; break_match; simpl; auto.
+  rewrite IHm. repeat break_if; auto; omega.
+Qed.
+
+Lemma compile_lift' :
+  forall l ty (e : S.expr l ty) ty' n,
+    compile (S.lift'(ty' := ty') n e) = U.shift' n (compile e).
+Proof.
+  refine (S.expr_mut_rect' _ _ _ _ _ _); intros; simpl.
+  - rewrite member_insert_member.
+    break_if; auto.
+  - f_equal.
+    apply H with (n := (S n)).
+  - f_equal; auto.
+  - unfold constr_name.
+    destruct c; repeat dependent destruction H; simpl; auto using f_equal, f_equal2.
+  - unfold elim_to_type_name.
+    destruct e; repeat dependent destruction H; simpl; auto using f_equal, f_equal2.
+Qed.
+
+Lemma compile_lift :
+  forall l ty ty' (e : S.expr l ty),
+    compile (S.lift ty' ty e) = U.shift (compile e).
+Proof.
+  intros.
+  apply compile_lift'.
+Qed.
+
+Lemma map_hmap_simple :
+  forall A (B : A -> Type) C D (f : forall a, B a -> C) (g : C -> D) l (hl : S.hlist B l),
+    map g (hmap_simple f hl) =
+    hmap_simple (fun a b => g (f a b)) hl.
+Proof.
+  induction hl; simpl; auto using f_equal.
+Qed.
+
+Lemma hmap_simple_hmap :
+  forall A (B C : A -> Type) D (f : forall a, B a -> C a) (g : forall a, C a -> D) l (hl : S.hlist B l),
+    hmap_simple g (S.hmap f hl) = hmap_simple (fun a b => g a (f a b)) hl.
+Proof.
+  induction hl; simpl; auto using f_equal.
+Qed.
+
+Lemma hmap_simple_ext :
+  forall A (B : A -> Type) C (f g : forall a, B a -> C) l (hl : S.hlist B l),
+    (forall a (b : B a), f a b = g a b) ->
+    hmap_simple f hl = hmap_simple g hl.
+Proof.
+  induction hl; simpl; auto using f_equal2.
+Qed.
+
+Theorem compile_subst :
+  forall l ty (e : S.expr l ty) l' (h : S.hlist (S.expr l') l),
+    compile (S.subst e h) = U.multisubst' (hmap_simple (@compile l') h) (compile e).
+Proof.
+  refine (S.expr_mut_rect' _ _ _ _ _ _); intros; simpl.
+  - now rewrite nth_member_hget.
+  - f_equal. rewrite H. simpl. f_equal. f_equal.
+    rewrite map_hmap_simple, hmap_simple_hmap.
+    apply hmap_simple_ext.
+    intros. apply compile_lift.
+  - f_equal; auto.
+  - unfold constr_name.
+    destruct c; repeat dependent destruction H; simpl; auto using f_equal, f_equal2.
+  - unfold elim_to_type_name.
+    destruct e; repeat dependent destruction H; simpl; auto using f_equal, f_equal2.
+Qed.
